\documentclass[11pt, fleqn]{article}

\usepackage[letterpaper, margin=0.7in]{geometry}
\usepackage{graphicx}
\usepackage{subcaption}
\usepackage{cleveref}
\usepackage{listings}
\usepackage{multicol}
\usepackage{tikz}
\usepackage{bm}
\usepackage{minted}
\usetikzlibrary{arrows}
\usepackage{wrapfig}
\usepackage{amsmath}
\usepackage{amssymb}
\usepackage[section]{placeins}
\usepackage{pgfplots,wrapfig}  
\pgfplotsset{compat=newest} 
\pgfplotsset{plot coordinates/math parser=false} 
\newlength\figureheight 
\newlength\figurewidth 
\setlength{\parindent}{0pt}
\newcommand\tab[1][1cm]{\hspace*{#1}}
\usepackage{algorithm}
\usepackage[noend]{algpseudocode}
\raggedbottom

\begin{document}

\begin{center}

\Large{COMP6212 Assignment 2 : Shakib-Bin Hamid 25250094 sh3g12}

\end{center}

\section{Black Scholes Equation Check Solution Correctness}

\subsection{}
Cumulative normal distribution function, $\mathcal{N}(x) = \frac{1}{\sqrt{2\pi}} \int_x^{-\infty} exp(\frac{-y^2}{2})dy$. $\mathcal{N}'(x) = \frac{1}{\sqrt{2\pi}}exp(\frac{-x^2}{2})$.

\subsection{}
\vspace{-1cm}
\begin{eqnarray*}
&& d_2 = d_1 - \sigma\sqrt{T-t}\\
&\implies& \frac{d_2^2}{2} = \frac{d_1^2}{2} + \frac{\sigma^2(T-t)}{2} - d_1\sigma\sqrt{T-t}\\
&\implies& \frac{d_1^2}{2} - \frac{d_2^2}{2} = d_1\sigma\sqrt{T-t} - \frac{\sigma^2(T-t)}{2} = log(\frac{S}{K}) + r(T-t)\\
&\implies& log(\frac{S}{K}) = \frac{d_1^2}{2} - \frac{d_2^2}{2} - r(T-t)\\
&\implies& \frac{S}{K} = exp(\frac{d_1^2}{2} - \frac{d_2^2}{2} - r(T-t)) = \frac{exp(\frac{-d_2^2}{2})}{exp(\frac{-d_1^2}{2} - r(T-t))} = \frac{\mathcal{N}'(d_2)}{\mathcal{N}'(d_1)exp(r(T-t))}\\
&\implies& S\mathcal{N}'(d_1) = Kexp(-r(T-t))\mathcal{N}'(d_2) 
\end{eqnarray*}

\subsection{}
\vspace{-1cm}
\begin{eqnarray*}
&& d_1 = \frac{log(\frac{S}{K})+(r+\frac{\sigma^2}{2})(T-t)}{\sigma\sqrt{(T-t)}} \\
&\implies& \frac{\partial d_1}{\partial S} = \frac{1}{\sigma\sqrt{(T-t)}} \frac{\partial}{\partial S}(logS - logK + (r+\frac{\sigma^2}{2})(T-t)) = \frac{1}{\sigma S \sqrt{(T-t)}}\\
&Similarly& d_2 = d_1 - \sigma\sqrt{T-t} \implies \frac{\partial d_2}{\partial S} = \frac{\partial d_1}{\partial S}= \frac{1}{\sigma S \sqrt{(T-t)}}
\end{eqnarray*}

\subsection{}
\vspace{-1cm}
\begin{eqnarray*}
&& c = S\mathcal{N}(d_1) - Kexp(-r(T-t))\mathcal{N}(d_2) \\
&\implies& \frac{\partial c}{\partial S} = \mathcal{N}(d_1) + \frac{1}{\sigma S \sqrt{(T-t)}}[S\mathcal{N}'(d_1) - Kexp(-r(T-t))\mathcal{N}'(d_2)] = \mathcal{N}(d_1)
\end{eqnarray*}
The above follows because -
\begin{eqnarray*}
Kexp(-r(T-t))\mathcal{N}'(d_2) &=& Kexp(-r(T-t))\mathcal{N}'(d_1 - \sigma\sqrt{T-t})\\
&=& Kexp(-r(T-t))\frac{1}{\sqrt{2\pi}}exp(\frac{-(d_1 - \sigma\sqrt{T-t})^2}{2})\\
&=& Kexp(-r(T-t))\frac{1}{\sqrt{2\pi}}exp(\frac{-d_1^2}{2})exp(\frac{2d_1\sigma\sqrt{T-t} - \sigma^2(T-t)}{2})\\
&=& Kexp(-r(T-t))\mathcal{N}'(d_1)exp(d_1\sigma\sqrt{T-t})exp(-\sigma^2(T-t))\\
&=& K\mathcal{N}'(d_1)exp(-r(T-t)-\frac{\sigma^2(T-t)}{2} + log(\frac{S}{K}) + r(T-t) + \frac{\sigma^2(T-t)}{2})\\
&=& K\mathcal{N}'(d_1)\frac{S}{K} = S\mathcal{N}'(d_1)
\end{eqnarray*}

\subsection{}
$
\frac{\partial c}{\partial S} = \mathcal{N}(d_1)
\implies \frac{\partial^2 c}{\partial S^2} = \mathcal{N}(d_1)\frac{\partial d_1}{\partial S} = \mathcal{N}(d_1)\frac{1}{\sigma S \sqrt{(T-t)}}
$






































\end{document}











